cleanup

LLVM_DS_RBT/Delete/Delete.thy
@@ -1,6 +1,7 @@
 theory Delete
   imports 
     Balance_LR
+    Combine
 begin
 
 
@@ -11,50 +12,178 @@ interpretation llvm_prim_arith_setup .
 interpretation llvm_prim_setup .
 
 
-subsection \<open>random crap\<close>
+fun rbt_del_ad where
+  "rbt_del_ad x rbt.Empty = rbt.Empty"
+| "rbt_del_ad x (rbt.Branch c a y s b) = 
+(
+  if x < y then
+    if is_black_b a
+    then rbt_balance_left (rbt_del_ad x a) y s b
+    else rbt.Branch color.R (rbt_del_ad x a) y s b
+  else if x > y then
+    if is_black_b b
+    then rbt_balance_right a y s (rbt_del_ad x b)
+    else rbt.Branch color.R a y s (rbt_del_ad x b)
+  else
+    rbt_combine a b
+)
+"
 
 
-definition "Equiv (f:: real \<Rightarrow> real) g \<equiv> \<forall>x. f (g x) = x"
+(*looks easy now but really wasn't*)
+lemma 
+  rbt_del_ad_correct_left:
+  "\<lbrakk>x < y\<rbrakk> \<Longrightarrow>
+  rbt_del_ad x (rbt.Branch c a (y::'k) (s::'a) b) = rbt_del_from_left x a y s b" and
+
+  rbt_del_ad_correct_right:
+  "\<lbrakk>x > y\<rbrakk> \<Longrightarrow>
+  rbt_del_ad x (rbt.Branch c a y s b) = rbt_del_from_right x a y s b" and
+
+  rbt_del_ad_correct:
+  "rbt_del_ad x (t:: ('k, 'a) rbt) = rbt_del x t"
+
+proof (induct x a y s b and x a y s b and x t
+    rule: rbt_del_from_left_rbt_del_from_right_rbt_del.induct)
+  case (2 x c a y s b)
+  then show ?case by (cases "x<y", auto)
+qed auto
 
 
-lemma 1 [intro]: "f = (\<lambda>x. f' (x - c)) \<Longrightarrow> Equiv f' g \<Longrightarrow> Equiv f (\<lambda>x. g x + c)"
-  unfolding Equiv_def by simp
+partial_function (M) del ::
+  "'ki \<Rightarrow> ('ki, 'v::llvm_rep) rbti \<Rightarrow> (('ki, 'v::llvm_rep) rbti) llM" where
+ "del x t_p = do {
+  if t_p = null then return null
+  else do {
+    t \<leftarrow> ll_load t_p;
+    case t of (RBT_NODE c a y s b) \<Rightarrow>
+    do {
+      le \<leftarrow> lt_impl x y;
+      if le = 1 then
+      do {
+        cond \<leftarrow> is_black_b_i a;
+        l_del \<leftarrow> del x a;
+        if cond = 1
+        then do { ll_free t_p; balance_left l_del y s b }
+        else do { set_left_p l_del t_p; set_color_p 0 t_p; return t_p }
+      }
+      else
+      do {
+        ge \<leftarrow> lt_impl y x;
+        if ge = 1
+        then do {
+          cond \<leftarrow> is_black_b_i b;
+          r_del \<leftarrow> del x b;
+          if cond = 1
+          then do { ll_free t_p; balance_right a y s (r_del) }
+          else do { set_right_p r_del t_p; set_color_p 0 t_p; return t_p }
+        }
+        else do {
+          key_delete y;          
+          ll_free t_p;
+          combine a b
+        }
+      }
+    }
+  }
+}"
 
-lemma 2 [intro]: "Equiv f (\<lambda>x. g x + (-c)) \<Longrightarrow> Equiv f (\<lambda>x. g x - c)"
-  by simp
 
-lemma 3 [intro]: "c \<noteq> 0 \<Longrightarrow> f = (\<lambda>x. f' ( x / c)) \<Longrightarrow> Equiv f' g \<Longrightarrow> Equiv f (\<lambda>x. c * g x)"
-  unfolding Equiv_def
-  by auto
+lemma del_correct':
+"
+  llvm_htriple
+  (\<upharpoonleft>key_assn k ki ** \<upharpoonleft>rbt_assn t ti)
+  (del ki ti)
+  (\<lambda>r. \<upharpoonleft>rbt_assn (rbt_del_ad k t) r ** \<upharpoonleft>key_assn k ki)
+"
+proof(induct k t arbitrary: ki ti rule: rbt_del_ad.induct)
+  case (1 x)
+  then show ?case
+    apply (subst del.simps)
+    apply vcg
+    done
+next
+  case (2 x c a y s b)
 
-lemma 4 [intro]: "f = (\<lambda>x. x) \<Longrightarrow> Equiv f (\<lambda>x. x)"
-  unfolding Equiv_def by simp
+  have IH1: 
+    "x < y \<Longrightarrow> llvm_htriple
+      (\<upharpoonleft>key_assn x ki \<and>* \<upharpoonleft>rbt_assn a ti)
+      (del ki ti)
+      (\<lambda>r. \<upharpoonleft>rbt_assn (rbt_del_ad x a) r \<and>* \<upharpoonleft>key_assn x ki)"
+    for ki ti
+    using 2(1-2) by fast
 
-lemma 5 [intro]: "Equiv f (\<lambda>x. (1/c) * g x ) \<Longrightarrow> Equiv f (\<lambda>x. g x / c)"
-  by simp
+  have IH2:
+    "y < x \<Longrightarrow> llvm_htriple
+      (\<upharpoonleft>key_assn x ki \<and>* \<upharpoonleft>rbt_assn b ti)
+      (del ki ti)
+      (\<lambda>r. \<upharpoonleft>rbt_assn (rbt_del_ad x b) r \<and>* \<upharpoonleft>key_assn x ki)"
+    for ki ti using 2(3-4) by fastforce
+
+  note [vcg_rules] = IH1 IH2
+
+  show ?case
+    apply (subst del.simps)
+    apply vcg (*x < y; is_black_b -- is automatic*)
+    subgoal (*x < y, \<not>is_black_b*)
+      apply auto
+      unfolding rbt_assn_branch_def
+      apply vcg
+      done 
+    subgoal (*x \<ge> y*)
+      apply vcg (*x > y; is_black_b -- is automatic*)
+      subgoal (*x > y; \<not>is_black_b*)
+        apply simp
+        unfolding rbt_assn_branch_def
+        apply vcg
+        done
+      subgoal (*x = y*) by vcg
+      done
+    done
+qed
 
 
+lemma del_correct:
+"
+  llvm_htriple
+  (\<upharpoonleft>key_assn k ki ** \<upharpoonleft>rbt_assn t ti)
+  (del ki ti)
+  (\<lambda>r. \<upharpoonleft>rbt_assn (rbt_del k t) r ** \<upharpoonleft>key_assn k ki)
+"
+  using del_correct' rbt_del_ad_correct by metis
 
-definition "g \<equiv> (\<lambda>(x::real). 2 * (x + 5 - x) + x + 12 * x - 1 + (1.1 * x))"
 
-schematic_goal "Equiv ?f g"
-  unfolding g_def
-  apply (rule | simp)+
+lemmas [llvm_code] = del.simps
+
+
+definition "delete x t \<equiv> do { 
+  del_res \<leftarrow> del x t;
+  (if del_res = null then return () else set_color_p 1 del_res);
+  return del_res 
+  }"
+
+
+lemma delete_correct [vcg_rules]:
+"
+  llvm_htriple
+  (\<upharpoonleft>key_assn k ki ** \<upharpoonleft>rbt_assn t ti)
+  (delete ki ti)
+  (\<lambda>r. \<upharpoonleft>rbt_assn (rbt_delete k t) r ** \<upharpoonleft>key_assn k ki)
+"
+  unfolding delete_def rbt_delete_def paint_def
+  supply del_correct[vcg_rules]
+  apply vcg
+  apply STATE_extract_pure
+  apply (erule rbt_assn_non_null_unfold, simp)
+  apply vcg
+  apply auto
+  unfolding rbt_assn_branch_def
+  apply vcg
   done
+(*this is me refusing to make a dedicated function that implements paint*)
 
 
-definition "Cond (ff::'a list \<Rightarrow> 'b) (gg:: 'a list \<Rightarrow> 'b) = (ff = gg)"
-
-
-lemma R1: "f [] = undefined \<Longrightarrow> (\<And>l. f l = E (hd l) (tl l)) \<Longrightarrow> Cond f (\<lambda>l. case l of x # xs \<Rightarrow> E x xs)" 
-  unfolding Cond_def
-  apply standard
-  by (simp add: list.case_eq_if)
-
-
-schematic_goal "Cond ?f (\<lambda>l. case l of x # (y # xs) \<Rightarrow> x)"
-  apply (rule R1)
-  sorry
+lemmas [llvm_code] = delete_def
 
 
 end 
