LLVM_DS_RBT/Setup.thy
@@ -4,6 +4,10 @@ theory Setup
     Abstract_Rbt
 begin
 
+
+subsection \<open>RBT_NODE Datatype\<close>
+
+
 datatype ('key :: llvm_rep, 'value :: llvm_rep) rbt_node =
   RBT_NODE
   (color: "8 word")
@@ -165,7 +169,9 @@ lemmas [llvm_inline] =
   rbt_node.right_def
 
 
-subsection \<open>Setters\<close>
+subsubsection \<open>Setters\<close>
+
+
 definition set_color :: 
   "('k::llvm_rep, 'v::llvm_rep) rbt_node \<Rightarrow> 8 word \<Rightarrow> _"
   where "set_color node col \<equiv> ll_insert_value node col 0"
@@ -212,6 +218,8 @@ lemmas [llvm_inline, simp] =
   set_right_p_def
 
 
+subsection \<open>Color Assertion\<close>
+
 
 fun color_assn' :: "color \<Rightarrow> 8 word \<Rightarrow> ll_assn" where
   "color_assn' color.R rep = \<up>(rep=0)"
@@ -227,12 +235,15 @@ lemma color_assn_eq: "\<upharpoonleft>color_assn c rep =
   by (cases c; simp)
 
 
+lemma color_assn_pure [is_pure_rule]: "is_pure color_assn" 
+  unfolding is_pure_def color_assn_eq by simp
+
+
 lemma [simp]: "\<upharpoonleft>color_assn color.R rep = \<up>(rep=0)"
   unfolding color_assn_def by simp
 
 lemma [simp]: "\<upharpoonleft>color_assn color.B rep = \<up>(rep=1)"
   unfolding color_assn_def by simp
-
 
 lemma [simp]: "\<upharpoonleft>color_assn c 0 = \<up>(c = color.R)"
   unfolding color_assn_eq
@@ -243,13 +254,11 @@ lemma [simp]: "\<upharpoonleft>color_assn c 1 = \<up>(c = color.B)"
   by (cases c; auto)
 
 
-
 lemma [simp]: "\<upharpoonleft>\<^sub>pcolor_assn color.R rep = \<up>(rep=0)"
   by (simp add: dr_assn_pure_prefix_def)
 
 lemma [simp]: "\<upharpoonleft>\<^sub>pcolor_assn color.B rep = \<up>(rep=1)"
   by (simp add: dr_assn_pure_prefix_def)
-
 
 lemma [simp]: "\<upharpoonleft>\<^sub>pcolor_assn c 0 = \<up>(c = color.R)"
   by (cases c; auto)
@@ -259,11 +268,12 @@ lemma [simp]: "\<upharpoonleft>\<^sub>pcolor_assn c 1 = \<up>(c = color.B)"
 
 
 lemma [simp]: "\<flat>\<^sub>pcolor_assn color.R rep = (rep=0)"
-  sorry
+  unfolding dr_assn_pure_asm_prefix_def
+  using color_assn_pure by auto
   
-
 lemma [simp]: "\<flat>\<^sub>p color_assn color.B rep = (rep=1)"
-  sorry
+  unfolding dr_assn_pure_asm_prefix_def
+  using color_assn_pure by auto
 
 lemma [simp]: "\<flat>\<^sub>pcolor_assn c 0 = (c = color.R)"
   by (cases c; auto)
@@ -272,24 +282,21 @@ lemma [simp]: "\<flat>\<^sub>pcolor_assn c 1 = (c = color.B)"
   by (cases c; auto)
 
 
-lemma color_assn_pure [is_pure_rule]: "is_pure color_assn"
-  unfolding is_pure_def
-proof(standard+)
-  fix col coli
-  show "sep_is_pure_assn (\<upharpoonleft>color_assn col coli)"
-    by (cases col; auto)
-qed
+subsection \<open>fb Setup\<close>
 
 
 definition fb :: "bool \<Rightarrow> 1 word" where "fb = from_bool"
+
 
 lemma fb_true [simp]: "fb True = 1" 
   unfolding fb_def
   by simp
 
+
 lemma fb_false [simp]: "fb False = 0" 
   unfolding fb_def
   by simp
+
 
 lemma fb_num [simp]: 
   "fb x = 0 \<longleftrightarrow> \<not>x"
@@ -297,8 +304,12 @@ lemma fb_num [simp]:
   unfolding fb_def
   by simp+
 
+
 abbreviation ll_True :: "1 word" where "ll_True \<equiv> 1"
 abbreviation ll_False :: "1 word" where "ll_False \<equiv> 0"
+
+
+subsection \<open>Linorder Locale\<close>
 
 
 locale linorder_impl =
@@ -312,6 +323,9 @@ locale linorder_impl =
               \<up>(r = fb (lhs < rhs)) **
               \<upharpoonleft>elem_assn lhs lhsi **
               \<upharpoonleft>elem_assn rhs rhsi)"
+
+
+subsection \<open>RBT Locale\<close>
 
 
 locale rbt_impl = linorder_impl lt_impl key_assn
@@ -330,10 +344,8 @@ interpretation llvm_prim_ctrl_setup .
 interpretation llvm_prim_arith_setup .
 interpretation llvm_prim_setup .
 
-datatype ('kk, 'vv) Conc = U | B "('kk, 'vv) rbt_node"
 
-
-datatype ('kk, 'vv) RbtA = RBTA "('kk, 'vv) rbti" "('kk, 'vv) Conc"
+subsection \<open>RBT Assertion\<close>
 
 
 fun rbt_assn' :: "
@@ -427,68 +439,17 @@ lemma rbt_assn_branch_def: "\<upharpoonleft>rbt_assn (Branch col lhs k v rhs) p 
   unfolding rbt_assn_def
   by simp
 
-subsection \<open>Foldable rbt assn\<close>
-
-
-fun rbt_assn_m' ::
-  "('k, 'v) rbt \<Rightarrow>
-  ('ki::llvm_rep, 'v::llvm_rep) RbtA \<Rightarrow>
-  ll_assn" where
-  "rbt_assn_m' rbt.Empty (RBTA p X) = \<up>(p = null)"
-| "rbt_assn_m' (rbt.Branch col lhs k v rhs) (RBTA p U) = 
-  (  
-    EXS coli lhsi ki vi rhsi. 
-          \<upharpoonleft>ll_bpto (RBT_NODE coli lhsi ki vi rhsi) p **
-          \<upharpoonleft>color_assn col coli **
-          \<upharpoonleft>rbt_assn lhs lhsi **
-          \<upharpoonleft>key_assn k ki **
-          \<up>(vi=v) **
-          \<upharpoonleft>rbt_assn rhs rhsi
-  )"
-| "rbt_assn_m' (rbt.Branch col lhs k v rhs) (RBTA p (B (RBT_NODE coli lhsi ki vi rhsi))) =
-  (    
-    \<upharpoonleft>ll_bpto (RBT_NODE coli lhsi ki vi rhsi) p **
-    \<upharpoonleft>color_assn col coli **
-    \<upharpoonleft>rbt_assn lhs lhsi **
-    \<upharpoonleft>key_assn k ki **
-    \<up>(vi=v) **
-    \<upharpoonleft>rbt_assn rhs rhsi
-  )  
-"
-
-
-definition "rbt_assn_m = mk_assn rbt_assn_m'"
-
-
-lemma rbt_assn_m_tag_def: "\<upharpoonleft>rbt_assn_m = rbt_assn_m'"
-  unfolding rbt_assn_m_def dr_assn_prefix_def mk_assn_def
-  by simp
-
-
-lemma close_rbt_assn_m_entails:
-  "
-  (
-    \<upharpoonleft>ll_bpto (RBT_NODE 0 lhsi ki vi rhsi) ti **
-    \<upharpoonleft>rbt_assn lhs lhsi **
-    \<upharpoonleft>key_assn k ki **
-    \<upharpoonleft>rbt_assn rhs rhsi
-  ) \<turnstile>
-  (\<upharpoonleft>rbt_assn_m (rbt.Branch color.R lhs k vi rhs) (RBTA ti (B (RBT_NODE 0 lhsi ki vi rhsi))))
-  "
-  unfolding rbt_assn_m_tag_def
-  by (simp add: sep_algebra_simps)
-
 
 lemma close_rbt_assn_entails:
   "
   (
-    \<upharpoonleft>ll_bpto (RBT_NODE ci lhsi ki vi rhsi) ti **
-    \<upharpoonleft>color_assn c ci **  
+    \<upharpoonleft>ll_bpto (RBT_NODE coli lhsi ki vi rhsi) ti **
+    \<upharpoonleft>color_assn col coli **  
     \<upharpoonleft>rbt_assn lhs lhsi **
     \<upharpoonleft>key_assn k ki **
     \<upharpoonleft>rbt_assn rhs rhsi
   ) \<turnstile> 
-  \<upharpoonleft>rbt_assn (rbt.Branch c lhs k vi rhs) ti
+  \<upharpoonleft>rbt_assn (rbt.Branch col lhs k vi rhs) ti
   "
   unfolding rbt_assn_branch_def
   apply (rule ENTAILSD)
@@ -517,13 +478,11 @@ lemma entails_to_ENTAILS_elim:
   using ENTAILS_def gen_drule by blast
 
 
-lemmas close_rbt_m_assn = entails_to_state_elim[OF close_rbt_assn_m_entails]
 lemmas close_rbt_assn = entails_to_state_elim[OF close_rbt_assn_entails]
                         entails_to_ENTAILS_elim[OF close_rbt_assn_entails]
 
 
-subsection \<open>rest\<close>
-
+subsection \<open>RBT Load Rule\<close>
 
 
 lemma load_rbt [vcg_rules]:
@@ -544,6 +503,9 @@ lemma load_rbt [vcg_rules]:
   "
   unfolding rbt_assn_branch_def
   by vcg
+
+
+subsection "Empty Function"
 
 
 definition empty :: "('ki, 'v) rbti llM"
