LLVM_DS_RBT/Export.thy
@@ -22,21 +22,18 @@ global_interpretation unat_rbt: rbt_impl
   key_delete 
   defines 
     unat_rbt_naive_insert = unat_rbt.naive_insert and
-    unat_rbt_balance = unat_rbt.balance and
     unat_rbt_insert = unat_rbt.insert and
     unat_rbt_empty = unat_rbt.empty and
     unat_rbt_lookup = unat_rbt.lookup and
     unat_rbt_free = unat_rbt.free and
-    unat_rbt_balance_left = unat_rbt.balance_left and
-    unat_rbt_balance_right = unat_rbt.balance_right
+    unat_rbt_delete = unat_rbt.delete
 proof(standard, goal_cases)
   case (1 lhs lhsi rhs rhsi)
-
   thus ?case
     apply vcg
-    unfolding bool.assn_def 
+    unfolding bool.assn_def
     apply (auto simp add: word1_neqZ_is_one word1_neq1_is_zero)
-     apply vcg+
+     apply vcg
     done
 next
   case (2 k ki)
@@ -55,10 +52,6 @@ abbreviation unat_rbt_insert_64 ::
   "_ \<Rightarrow> _ \<Rightarrow> (64 word, 8 word) rbt_node ptr \<Rightarrow> _"        
   where "unat_rbt_insert_64 \<equiv> unat_rbt_insert"
 
-abbreviation unat_rbt_balance_64 :: 
-  "(64 word, 8 word) rbt_node ptr \<Rightarrow> _"        
-  where "unat_rbt_balance_64 \<equiv> unat_rbt_balance"
-
 abbreviation unat_rbt_empty_64 :: "(64 word, 8 word) rbti llM"
   where "unat_rbt_empty_64 \<equiv> unat_rbt_empty"
 
@@ -68,21 +61,17 @@ abbreviation unat_rbt_lookup_64 :: "(64 word, 8 word) rbti \<Rightarrow> _"
 abbreviation unat_rbt_free_64 :: "(64 word, 8 word) rbti \<Rightarrow> _"
   where "unat_rbt_free_64 \<equiv> unat_rbt_free"
 
-abbreviation unat_rbt_balance_left_64 :: "(64 word, 8 word) rbti \<Rightarrow> _"
-  where "unat_rbt_balance_left_64 \<equiv> unat_rbt_balance_left"
+abbreviation unat_rbt_delete_64 :: "_ \<Rightarrow> (64 word, 8 word) rbti \<Rightarrow> _"
+  where "unat_rbt_delete_64 \<equiv> unat_rbt_delete"
 
-abbreviation unat_rbt_balance_right_64 :: "(64 word, 8 word) rbti \<Rightarrow> _"
-  where "unat_rbt_balance_right_64 \<equiv> unat_rbt_balance_right"
 
 export_llvm
   unat_rbt_empty_64 is "rbt_node* rbt_empty()"  
   unat_rbt_naive_insert_64 is "rbt_node* rbt_naive_insert(rbt_node*, uint64_t, uint8_t)"
   unat_rbt_insert_64 is "rbt_node* rbt_insert(uint64_t, uint8_t, rbt_node*)"
-  unat_rbt_balance_64 is "rbt_node* rbt_balance(rbt_node*, uint64_t, uint8_t, rbt_node*)"
   unat_rbt_lookup_64 is "option_i* rbt_lookup(rbt_node*, uint64_t)"
   unat_rbt_free_64 is "void rbt_free(rbt_node*)"
-  unat_rbt_balance_left_64 is "rbt_node* rbt_balance_left(rbt_node*, uint64_t, uint8_t, rbt_node*)"
-  unat_rbt_balance_right_64 is "rbt_node* rbt_balance_right(rbt_node*, uint64_t, uint8_t, rbt_node*)"
+  unat_rbt_delete_64 is "rbt_node* rbt_delete(uint64_t, rbt_node*)"
   defines \<open>
     typedef struct {
        uint8_t color;
