LLVM_DS_RBT/Insert/Balance_Foldable.thy
@@ -1,0 +1,40 @@
+theory Balance_Foldable
+  imports 
+    Balance
+    "../Setup_Foldable"
+begin
+
+
+context rbt_impl
+begin
+interpretation llvm_prim_ctrl_setup .
+interpretation llvm_prim_arith_setup .
+interpretation llvm_prim_setup .
+
+
+lemma assn_ent_assnm: "\<upharpoonleft>rbt_assn t ti = \<upharpoonleft>rbt_assn_m t (RBTA ti U)"
+unfolding rbt_assn_m_tag_def rbt_assn_tag_def
+  apply (induction t)
+  apply auto
+  unfolding rbt_assn_tag_def
+  by auto
+
+
+lemma balance_correct_ :
+  "llvm_htriple
+  (
+    \<upharpoonleft>rbt_assn_m tree_l (RBTA tree_li X) **
+    \<upharpoonleft>rbt_assn_m tree_r (RBTA tree_ri Y) **   
+    \<upharpoonleft>key_assn k ki
+  )
+  (balance tree_li ki v tree_ri)
+  (\<lambda>ri. \<upharpoonleft>rbt_assn (rbt_balance tree_l k v tree_r) ri) 
+  "
+  apply (rule htriple_ent_pre)
+  sorry
+
+
+end
+
+
+end
