LLVM_DS_RBT/Setup_Foldable.thy
@@ -1,0 +1,71 @@
+theory Setup_Foldable
+  imports Setup
+begin
+
+
+datatype ('kk, 'vv) Conc = U | B "('kk, 'vv) rbt_node"
+
+
+datatype ('kk, 'vv) RbtA = RBTA "('kk, 'vv) rbti" "('kk, 'vv) Conc"
+
+
+context rbt_impl
+begin
+interpretation llvm_prim_ctrl_setup .
+interpretation llvm_prim_arith_setup .
+interpretation llvm_prim_setup .
+
+
+fun rbt_assn_m' ::
+  "('k, 'v) rbt \<Rightarrow>
+  ('ki::llvm_rep, 'v::llvm_rep) RbtA \<Rightarrow>
+  ll_assn" where
+  "rbt_assn_m' rbt.Empty (RBTA p X) = \<up>(p = null)"
+| "rbt_assn_m' (rbt.Branch col lhs k v rhs) (RBTA p U) = 
+  (  
+    EXS coli lhsi ki vi rhsi. 
+          \<upharpoonleft>ll_bpto (RBT_NODE coli lhsi ki vi rhsi) p **
+          \<upharpoonleft>color_assn col coli **
+          \<upharpoonleft>rbt_assn lhs lhsi **
+          \<upharpoonleft>key_assn k ki **
+          \<up>(vi=v) **
+          \<upharpoonleft>rbt_assn rhs rhsi
+  )"
+| "rbt_assn_m' (rbt.Branch col lhs k v rhs) (RBTA p (B (RBT_NODE coli lhsi ki vi rhsi))) =
+  (    
+    \<upharpoonleft>ll_bpto (RBT_NODE coli lhsi ki vi rhsi) p **
+    \<upharpoonleft>color_assn col coli **
+    \<upharpoonleft>rbt_assn lhs lhsi **
+    \<upharpoonleft>key_assn k ki **
+    \<up>(vi=v) **
+    \<upharpoonleft>rbt_assn rhs rhsi
+  )  
+"
+
+
+definition "rbt_assn_m = mk_assn rbt_assn_m'"
+
+
+lemma rbt_assn_m_tag_def: "\<upharpoonleft>rbt_assn_m = rbt_assn_m'"
+  unfolding rbt_assn_m_def dr_assn_prefix_def mk_assn_def
+  by simp
+
+
+lemma close_rbt_assn_m_entails:
+  "
+  (
+    \<upharpoonleft>ll_bpto (RBT_NODE 0 lhsi ki vi rhsi) ti **
+    \<upharpoonleft>rbt_assn lhs lhsi **
+    \<upharpoonleft>key_assn k ki **
+    \<upharpoonleft>rbt_assn rhs rhsi
+  ) \<turnstile>
+  (\<upharpoonleft>rbt_assn_m (rbt.Branch color.R lhs k vi rhs) (RBTA ti (B (RBT_NODE 0 lhsi ki vi rhsi))))
+  "
+  unfolding rbt_assn_m_tag_def
+  by (simp add: sep_algebra_simps)
+
+
+end
+
+
+end
